wordarray: added shallow and value semantics embedding of mapAccum
Defined a shallow and value semantics of mapAccum for word arrays. Also
proved several helper lemmas about mapAccum for both the shallow and the
value semantics. Other changes are some minor proof clean up and
commenting out some outdated lemmas.

cogent/examples/wa_connect/WordArray_Abstractions.thy
@@ -299,6 +299,79 @@ definition wordarray_fold_no_break':
          (myslice (unat (WordArrayMapP.frm\<^sub>f x)) (unat (WordArrayMapP.to\<^sub>f x)) (WordArrayMapP.arr\<^sub>f x)) 
          (WordArrayMapP.acc\<^sub>f x)" 
 end
+
+
+fun mapAccum :: "('a \<Rightarrow> 'b  \<Rightarrow> ('c \<times> 'b)) \<Rightarrow> 'a list \<Rightarrow> 'b \<Rightarrow> ('c list \<times> 'b)"
+  where
+"mapAccum _ [] acc = ([], acc)" |
+"mapAccum f (x#xs) acc = 
+  (let (a, b) = f x acc;
+       (as, b') = mapAccum f xs b
+   in (a#as, b'))"
+
+fun listAccumStep :: "('a \<Rightarrow> 'b  \<Rightarrow> ('c \<times> 'b)) \<Rightarrow> 'a \<Rightarrow> ('c list \<times> 'b) \<Rightarrow> ('c list \<times> 'b)"
+  where
+"listAccumStep f x (ys, acc) = (let (y, acc') = f x acc in (ys @ [y], acc'))"
+
+lemma mapAccum_step:
+  "mapAccum f (xs @ [x]) acc = listAccumStep f x (mapAccum f xs acc)"
+  apply (induct arbitrary: x acc rule: list.induct)
+   apply clarsimp
+  apply (clarsimp split: prod.split)
+  done
+
+
+lemma mapAccum_length:
+  "length (prod.fst (mapAccum f xs acc)) = length xs"
+  apply (induct arbitrary: acc rule: rev_induct)
+   apply simp
+  apply (subst mapAccum_step)
+  apply clarsimp
+  apply (drule_tac x = acc in meta_spec)
+  by (metis (no_types, lifting) Product_Type.split_def fst_conv length_append_singleton listAccumStep.simps prod.collapse)
+
+
+
+lemma 
+  "map f xs = prod.fst (mapAccum (\<lambda>a b. (f a, b)) xs ())"
+  by (induct xs; clarsimp split: prod.split)
+
+lemma
+  "fold f xs acc = prod.snd (mapAccum (\<lambda>a b. (a, f a b)) xs acc)"
+  apply (induct rule: rev_induct; clarsimp split: prod.split)
+  apply (subst mapAccum_step)
+  by (metis (no_types, lifting) case_prod_beta listAccumStep.simps prod.collapse snd_conv)
+
+
+
+fun cogent_isa_pair :: "('a, 'b) RR \<Rightarrow> ('a \<times> 'b)"
+  where
+"cogent_isa_pair x = (RR.p1\<^sub>f x, RR.p2\<^sub>f x)"
+
+term "mapAccum 
+          (\<lambda>a b. cogent_isa_pair ((WordArrayMapP.f\<^sub>f x) (ElemAO.make a b (WordArrayMapP.obsv\<^sub>f x)))) 
+          (myslice (unat (WordArrayMapP.frm\<^sub>f x)) (unat (WordArrayMapP.to\<^sub>f x)) (WordArrayMapP.arr\<^sub>f x)) 
+          (WordArrayMapP.acc\<^sub>f x)"
+overloading
+  wordarray_map_no_break' \<equiv> wordarray_map_no_break
+begin
+definition wordarray_map_no_break':
+ "wordarray_map_no_break' (x :: ('a WordArray, 32 word, 32 word, ('a, 'acc, 'obsv) ElemAO \<Rightarrow> ('a, 'acc) RR, 'acc, 'obsv) WordArrayMapP) \<equiv> 
+    (let xs = List.take (unat (WordArrayMapP.frm\<^sub>f x)) (WordArrayMapP.arr\<^sub>f x);
+         zs = List.drop (unat (WordArrayMapP.to\<^sub>f x)) (WordArrayMapP.arr\<^sub>f x);
+        (ys, acc) = mapAccum 
+          (\<lambda>a b. cogent_isa_pair ((WordArrayMapP.f\<^sub>f x) (ElemAO.make a b (WordArrayMapP.obsv\<^sub>f x)))) 
+          (myslice (unat (WordArrayMapP.frm\<^sub>f x)) (unat (WordArrayMapP.to\<^sub>f x)) (WordArrayMapP.arr\<^sub>f x)) 
+          (WordArrayMapP.acc\<^sub>f x)
+    in RR.make (xs @ ys @ zs) acc)" 
+end
+
+
+
+
+
+
+
 context WordArray begin
 
 subsection "Level 0 \<xi> Abstractions"
@@ -347,10 +420,7 @@ fun \<xi>0 :: "(char list, atyp, 32 word) uabsfuns"
                  else False)))" 
 
 subsubsection "Value Semantics"
-\<comment>\<open> These definitions will have to change because for different word sizes because only using
-    @{term "VWA xs"} means we cannot determine what word array it is meant to represent in the case
-    that @{term "xs::(funtyp, vabstyp) vval list"} is empty. Either we need to define a new dataype
-    or we modify the current type to include the word type. \<close>
+
 definition val_wa_length
   where
   "val_wa_length x y = (\<exists>xs len t. x = VAbstract (VWA (TPrim (Num t)) xs) \<and> y = VPrim (LU32 len) \<and> 
@@ -449,17 +519,8 @@ declare upd_wa_foldnb_bod.simps[simp del]
 lemma upd_wa_foldnb_bod_to_geq_len:
   "\<lbrakk>upd_wa_foldnb_bod \<xi>\<^sub>u \<sigma> p frm len f acc obsv s (\<sigma>', r); \<sigma> p = option.Some (UAbstract (UWA t len arr));
     to \<ge> len\<rbrakk> \<Longrightarrow> upd_wa_foldnb_bod \<xi>\<^sub>u \<sigma> p frm to f acc obsv s (\<sigma>', r)"
-  apply (induct arbitrary: to arr t
-                rule: upd_wa_foldnb_bod.induct[where ?a0.0 = \<xi>\<^sub>u and
-                                                       ?a1.0 = \<sigma> and 
-                                                       ?a2.0 = p and 
-                                                       ?a3.0 = frm and 
-                                                       ?a4.0 = len and
-                                                       ?a5.0 = f and
-                                                       ?a6.0 = acc and
-                                                       ?a7.0 = obsv and
-                                                       ?a8.0 = s and
-                                                       ?a9.0 = "(\<sigma>', r)"])
+  apply (induct arbitrary: to arr t 
+                rule: upd_wa_foldnb_bod.induct[of _ \<xi>\<^sub>u \<sigma> p frm len f acc obsv s "(\<sigma>', r)"])
   apply clarsimp
   apply (drule_tac x = to in meta_spec)
   apply (subst (asm) upd_wa_foldnb_bod.simps)
@@ -507,16 +568,7 @@ lemma upd_wa_foldnb_bod_to_geq_len:
 lemma upd_wa_foldnb_bod_to_geq_lenD:
   "\<lbrakk>upd_wa_foldnb_bod \<xi>\<^sub>u \<sigma> p frm to f acc obsv s (\<sigma>', r); \<sigma> p = option.Some (UAbstract (UWA t len arr));
     to \<ge> len\<rbrakk> \<Longrightarrow> upd_wa_foldnb_bod \<xi>\<^sub>u \<sigma> p frm len f acc obsv s (\<sigma>', r)"
-  apply (induct rule: upd_wa_foldnb_bod.induct[where ?a0.0 = \<xi>\<^sub>u and
-                                                       ?a1.0 = \<sigma> and 
-                                                       ?a2.0 = p and 
-                                                       ?a3.0 = frm and 
-                                                       ?a4.0 = to and
-                                                       ?a5.0 = f and
-                                                       ?a6.0 = acc and
-                                                       ?a7.0 = obsv and
-                                                       ?a8.0 = s and 
-                                                       ?a9.0 = "(\<sigma>', r)"])
+  apply (induct rule: upd_wa_foldnb_bod.induct[of _ \<xi>\<^sub>u \<sigma> p frm to f acc obsv s "(\<sigma>', r)"])
   apply clarsimp
   apply (drule_tac x = len in meta_spec)
   apply (subst (asm) upd_wa_foldnb_bod.simps)
@@ -564,17 +616,8 @@ lemma upd_wa_foldnb_bod_step:
     ({p} \<union> s \<union> {arr + size_of_num_type t * i | i. i < len}) \<inter> w1 = {};
     \<xi>\<^sub>u, [URecord [(v, upd.uval_repr v), (r, upd.uval_repr r), (obsv, upd.uval_repr obsv)]] \<turnstile> (\<sigma>', App f (Var 0))\<Down>! (\<sigma>'', r')\<rbrakk> 
     \<Longrightarrow> upd_wa_foldnb_bod \<xi>\<^sub>u \<sigma> p frm (to + 1) f acc obsv s (\<sigma>'', r')"
-  apply (induct arbitrary: len arr v r r' \<sigma>' \<sigma>'' obsv s t w1 w2
-                rule: upd_wa_foldnb_bod.induct[where ?a0.0 = \<xi>\<^sub>u and
-                                                       ?a1.0 = \<sigma> and 
-                                                       ?a2.0 = p and 
-                                                       ?a3.0 = frm and 
-                                                       ?a4.0 = to and
-                                                       ?a5.0 = f and
-                                                       ?a6.0 = acc and
-                                                       ?a7.0 = obsv and
-                                                       ?a8.0 = s and 
-                                                       ?a9.0 = "(\<sigma>', r)"])
+  apply (induct arbitrary: len arr v r r' \<sigma>' \<sigma>'' t w1 w2
+                rule: upd_wa_foldnb_bod.induct[of _ \<xi>\<^sub>u \<sigma> p frm to f acc obsv s "(\<sigma>', r)"])
   apply clarsimp
   apply (drule_tac x = len in meta_spec)
   apply (erule upd_wa_foldnb_bod.elims)
@@ -588,8 +631,6 @@ lemma upd_wa_foldnb_bod_step:
    apply (drule_tac x = r' in meta_spec)
    apply (drule_tac x = a in meta_spec)
    apply (drule_tac x = \<sigma>'' in meta_spec)
-   apply (drule_tac x = obsv in meta_spec)
-   apply (drule_tac x = s in meta_spec)
    apply (drule_tac x = t in meta_spec)
    apply (drule_tac x = w1 in meta_spec)
    apply (drule_tac x = w2 in meta_spec)
@@ -658,16 +699,7 @@ lemma upd_wa_foldnb_bod_back_step':
     \<sigma> p = option.Some (UAbstract (UWA t len arr)); len < to\<rbrakk>
     \<Longrightarrow> upd_wa_foldnb_bod \<xi>\<^sub>u \<sigma> p frm (to - 1) f acc obsv s (\<sigma>', r)"
   apply (induct arbitrary: len arr t
-                rule: upd_wa_foldnb_bod.induct[where ?a0.0 = \<xi>\<^sub>u and
-                                                       ?a1.0 = \<sigma> and 
-                                                       ?a2.0 = p and 
-                                                       ?a3.0 = frm and 
-                                                       ?a4.0 = "to" and
-                                                       ?a5.0 = f and
-                                                       ?a6.0 = acc and
-                                                       ?a7.0 = obsv and
-                                                       ?a8.0 = s and
-                                                       ?a9.0 = "(\<sigma>', r)"]; clarsimp)
+                rule: upd_wa_foldnb_bod.induct[of _  \<xi>\<^sub>u \<sigma> p frm to f acc obsv s "(\<sigma>', r)"]; clarsimp)
   apply (drule_tac x = len in meta_spec)
   apply (erule upd_wa_foldnb_bod.elims)  
   apply (subst upd_wa_foldnb_bod.simps)
@@ -724,17 +756,8 @@ lemma upd_wa_foldnb_bod_back_step:
         (\<xi>\<^sub>u, [URecord [(v, upd.uval_repr v), (r'', upd.uval_repr r''), 
           (obsv, upd.uval_repr obsv)]] \<turnstile> (\<sigma>'', App f (Var 0))\<Down>! (\<sigma>', r)) \<and>
         frame \<sigma>'' w1 \<sigma>' w2 \<and> ({p} \<union> s \<union> {arr + size_of_num_type t * i | i. i < len}) \<inter> w1 = {}"
-  apply (induct arbitrary: len arr \<sigma>' r obsv s t
-                rule: upd_wa_foldnb_bod.induct[where ?a0.0 = \<xi>\<^sub>u and
-                                                       ?a1.0 = \<sigma> and 
-                                                       ?a2.0 = p and 
-                                                       ?a3.0 = frm and 
-                                                       ?a4.0 = "to" and
-                                                       ?a5.0 = f and
-                                                       ?a6.0 = acc and
-                                                       ?a7.0 = obsv and
-                                                       ?a8.0 = s and
-                                                       ?a9.0 = "(\<sigma>', r)"]; clarsimp)
+  apply (induct arbitrary: len arr \<sigma>' r t
+                rule: upd_wa_foldnb_bod.induct[of _ \<xi>\<^sub>u \<sigma> p frm to f acc obsv s "(\<sigma>', r)"]; clarsimp)
   apply (erule upd_wa_foldnb_bod.elims)  
   apply (clarsimp split: if_split_asm)
    apply (drule_tac x = len in meta_spec)
@@ -744,8 +767,6 @@ lemma upd_wa_foldnb_bod_back_step:
    apply (drule_tac x = arr in meta_spec)
    apply (drule_tac x = a in meta_spec)
    apply (drule_tac x = b in meta_spec)
-   apply (drule_tac x = obsv in meta_spec)
-   apply (drule_tac x = s in meta_spec)
    apply (drule_tac x = t in meta_spec)
    apply clarsimp
    apply (case_tac "frma < to"; clarsimp)
@@ -910,37 +931,30 @@ fun \<xi>1 :: "(char list, atyp, 32 word) uabsfuns"
 
 subsubsection "Value Semantics"
 
-type_synonym ('f, 'a) vfoldmapdef = "(char list, vatyp) vabsfuns \<Rightarrow> ('f, 'a) vval list \<Rightarrow> nat \<Rightarrow> 
+type_synonym ('f, 'a) vfoldmapdef = "(char list, vatyp) vabsfuns \<Rightarrow> type \<Rightarrow> ('f, 'a) vval list \<Rightarrow> nat \<Rightarrow> 
                                       nat \<Rightarrow> 'f expr \<Rightarrow> ('f, 'a) vval \<Rightarrow> ('f, 'a) vval \<Rightarrow> 
                                       ('f, 'a) vval \<Rightarrow> bool"
 
 function val_wa_foldnb_bod :: "(char list, vatyp) vfoldmapdef"
   where
-  "val_wa_foldnb_bod \<xi>\<^sub>v xs frm to f acc obsv res = 
+  "val_wa_foldnb_bod \<xi>\<^sub>v t xs frm to f acc obsv res = 
     (if frm < min to (length xs)
       then (\<exists>acc'. (\<xi>\<^sub>v, [(VRecord [xs ! frm, acc, obsv])] \<turnstile> App f (Var 0) \<Down> acc') \<and>
-          val_wa_foldnb_bod \<xi>\<^sub>v xs (Suc frm) to f acc' obsv res)
+          val_wa_foldnb_bod \<xi>\<^sub>v t xs (Suc frm) to f acc' obsv res)
     else acc = res)"
   by pat_completeness auto
 termination
-  apply (relation "measure (\<lambda>(_, _, frm, to, _, _, _, _). to - frm)"; clarsimp)
+  apply (relation "measure (\<lambda>(_, _, _, frm, to, _, _, _, _). to - frm)"; clarsimp)
   apply linarith
   done
 print_theorems
 declare val_wa_foldnb_bod.simps[simp del]
 
 lemma val_wa_foldnb_bod_append:
-  "\<lbrakk>to \<le> length xs; val_wa_foldnb_bod \<xi>\<^sub>v (xs @ [x]) frm to f acc obsv r\<rbrakk>
-    \<Longrightarrow> val_wa_foldnb_bod \<xi>\<^sub>v xs frm to f acc obsv r"
+  "\<lbrakk>to \<le> length xs; val_wa_foldnb_bod \<xi>\<^sub>v t (xs @ [x]) frm to f acc obsv r\<rbrakk>
+    \<Longrightarrow> val_wa_foldnb_bod \<xi>\<^sub>v t xs frm to f acc obsv r"
   apply (induct arbitrary: x 
-                rule: val_wa_foldnb_bod.induct[where ?a0.0 = \<xi>\<^sub>v and
-                                                       ?a1.0 = xs and
-                                                       ?a2.0 = frm and
-                                                       ?a3.0 = to and
-                                                       ?a4.0 = f and
-                                                       ?a5.0 = acc and
-                                                       ?a6.0 = obsv and
-                                                       ?a7.0 = r]; clarsimp)
+                rule: val_wa_foldnb_bod.induct[of _ \<xi>\<^sub>v t xs frm to f acc obsv r]; clarsimp)
   apply (erule val_wa_foldnb_bod.elims)
   apply (clarsimp split: if_splits)
    apply (drule_tac x = acc' in meta_spec)
@@ -955,18 +969,10 @@ lemma val_wa_foldnb_bod_append:
   done
 
 lemma val_wa_foldnb_bod_append_incl_to:
-  "\<lbrakk>frm < length (xs @ [x]); to > length xs; val_wa_foldnb_bod \<xi>\<^sub>v (xs @ [x]) frm to f acc obsv r\<rbrakk>
-    \<Longrightarrow> \<exists>r'. val_wa_foldnb_bod \<xi>\<^sub>v xs frm to f acc obsv r' \<and> (\<xi>\<^sub>v, [VRecord [x, r', obsv]] \<turnstile> (App f (Var 0)) \<Down> r)"
+  "\<lbrakk>frm < length (xs @ [x]); to > length xs; val_wa_foldnb_bod \<xi>\<^sub>v t (xs @ [x]) frm to f acc obsv r\<rbrakk>
+    \<Longrightarrow> \<exists>r'. val_wa_foldnb_bod \<xi>\<^sub>v t xs frm to f acc obsv r' \<and> (\<xi>\<^sub>v, [VRecord [x, r', obsv]] \<turnstile> (App f (Var 0)) \<Down> r)"
   apply (induct arbitrary: x
-                rule: val_wa_foldnb_bod.induct[where ?a0.0 = \<xi>\<^sub>v and
-                                                       ?a1.0 = xs and
-                                                       ?a2.0 = frm and
-                                                       ?a3.0 = to and
-                                                       ?a4.0 = f and
-                                                       ?a5.0 = acc and
-                                                       ?a6.0 = obsv and
-                                                       ?a7.0 = r])
-  apply clarsimp
+                rule: val_wa_foldnb_bod.induct[of _ \<xi>\<^sub>v t xs frm to f acc obsv r]; clarsimp)
   apply (case_tac "frm = length xs")
    apply (subst val_wa_foldnb_bod.simps)
    apply clarsimp
@@ -988,19 +994,11 @@ lemma val_wa_foldnb_bod_append_incl_to:
   done
 
 lemma val_wa_foldnb_bod_step:
-  "\<lbrakk>val_wa_foldnb_bod \<xi>\<^sub>v xs frm to f acc obsv r; frm \<le> to; to < length xs; 
+  "\<lbrakk>val_wa_foldnb_bod \<xi>\<^sub>v t xs frm to f acc obsv r; frm \<le> to; to < length xs; 
     \<xi>\<^sub>v, [VRecord [xs ! to, r, obsv]] \<turnstile> (App f (Var 0)) \<Down> (r')\<rbrakk> 
-    \<Longrightarrow> val_wa_foldnb_bod \<xi>\<^sub>v xs frm (Suc to) f acc obsv r'"
+    \<Longrightarrow> val_wa_foldnb_bod \<xi>\<^sub>v t xs frm (Suc to) f acc obsv r'"
   apply (induct arbitrary: r'
-                rule: val_wa_foldnb_bod.induct[where ?a0.0 = \<xi>\<^sub>v and
-                                                       ?a1.0 = xs and 
-                                                       ?a2.0 = frm and 
-                                                       ?a3.0 = to and 
-                                                       ?a4.0 = f and
-                                                       ?a5.0 = acc and
-                                                       ?a6.0 = obsv and
-                                                       ?a7.0 = r])
-  apply clarsimp
+                rule: val_wa_foldnb_bod.induct[of _ \<xi>\<^sub>v t xs frm to f acc obsv r]; clarsimp)
   apply (erule val_wa_foldnb_bod.elims)
   apply (clarsimp split: if_split_asm)
    apply (drule_tac x = acc' in meta_spec)
@@ -1018,16 +1016,9 @@ lemma val_wa_foldnb_bod_step:
   done
 
 lemma val_wa_foldnb_bod_to_geq_len:
-  "\<lbrakk>val_wa_foldnb_bod \<xi>\<^sub>v xs frm (length xs) f acc obsv r; length xs \<le> to\<rbrakk> 
-    \<Longrightarrow> val_wa_foldnb_bod \<xi>\<^sub>v xs frm to f acc obsv r"
-  apply (induct rule: val_wa_foldnb_bod.induct[where ?a0.0 = \<xi>\<^sub>v and
-                                                       ?a1.0 = xs and 
-                                                       ?a2.0 = frm and 
-                                                       ?a3.0 = to  and 
-                                                       ?a4.0 = f and
-                                                       ?a5.0 = acc and
-                                                       ?a6.0 = obsv and
-                                                       ?a7.0 = r]; clarsimp)
+  "\<lbrakk>val_wa_foldnb_bod \<xi>\<^sub>v t xs frm (length xs) f acc obsv r; length xs \<le> to\<rbrakk> 
+    \<Longrightarrow> val_wa_foldnb_bod \<xi>\<^sub>v t xs frm to f acc obsv r"
+  apply (induct rule: val_wa_foldnb_bod.induct[of _ \<xi>\<^sub>v t xs frm to f acc obsv r]; clarsimp)
   apply (erule val_wa_foldnb_bod.elims)
   apply (clarsimp split: if_split_asm)
    apply (erule_tac x = acc' in meta_allE; clarsimp)
@@ -1040,16 +1031,9 @@ lemma val_wa_foldnb_bod_to_geq_len:
   done
 
 lemma val_wa_foldnb_bod_to_geq_lenD:
-  "\<lbrakk>val_wa_foldnb_bod \<xi>\<^sub>v xs frm to f acc obsv r; length xs \<le> to\<rbrakk> 
-    \<Longrightarrow> val_wa_foldnb_bod \<xi>\<^sub>v xs frm (length xs) f acc obsv r"
-  apply (induct rule: val_wa_foldnb_bod.induct[where ?a0.0 = \<xi>\<^sub>v and
-                                                       ?a1.0 = xs and 
-                                                       ?a2.0 = frm and 
-                                                       ?a3.0 = to and 
-                                                       ?a4.0 = f and
-                                                       ?a5.0 = acc and
-                                                       ?a6.0 = obsv and
-                                                       ?a7.0 = r]; clarsimp)
+  "\<lbrakk>val_wa_foldnb_bod \<xi>\<^sub>v t xs frm to f acc obsv r; length xs \<le> to\<rbrakk> 
+    \<Longrightarrow> val_wa_foldnb_bod \<xi>\<^sub>v t xs frm (length xs) f acc obsv r"
+  apply (induct rule: val_wa_foldnb_bod.induct[of _ \<xi>\<^sub>v t xs frm to f acc obsv r]; clarsimp)
   apply (erule val_wa_foldnb_bod.elims)
   apply (clarsimp split: if_split_asm)
    apply (erule_tac x = acc' in meta_allE; clarsimp)
@@ -1062,16 +1046,9 @@ lemma val_wa_foldnb_bod_to_geq_lenD:
   done
 
 lemma val_wa_foldnb_bod_back_step':
-  "\<lbrakk>val_wa_foldnb_bod \<xi>\<^sub>v xs frm (Suc to) f acc obsv r; length xs < Suc to\<rbrakk>
-    \<Longrightarrow> val_wa_foldnb_bod \<xi>\<^sub>v xs frm to f acc obsv r"
-  apply (induct rule: val_wa_foldnb_bod.induct[where ?a0.0 = \<xi>\<^sub>v and
-                                                       ?a1.0 = xs and 
-                                                       ?a2.0 = frm and 
-                                                       ?a3.0 = to  and 
-                                                       ?a4.0 = f and
-                                                       ?a5.0 = acc and
-                                                       ?a6.0 = obsv and
-                                                       ?a7.0 = r]; clarsimp)
+  "\<lbrakk>val_wa_foldnb_bod \<xi>\<^sub>v t xs frm (Suc to) f acc obsv r; length xs < Suc to\<rbrakk>
+    \<Longrightarrow> val_wa_foldnb_bod \<xi>\<^sub>v t xs frm to f acc obsv r"
+  apply (induct rule: val_wa_foldnb_bod.induct[of _ \<xi>\<^sub>v t xs frm to f acc obsv r]; clarsimp)
   apply (erule val_wa_foldnb_bod.elims)
   apply (clarsimp split: if_split_asm)
    apply (erule_tac x = acc' in meta_allE; clarsimp)
@@ -1084,18 +1061,10 @@ lemma val_wa_foldnb_bod_back_step':
   done
 
 lemma val_wa_foldnb_bod_back_step:
-  "\<lbrakk>val_wa_foldnb_bod \<xi>\<^sub>v xs frm (Suc to) f acc obsv r; Suc to \<le> length xs; frm < Suc to\<rbrakk>
-    \<Longrightarrow> \<exists>r'. val_wa_foldnb_bod \<xi>\<^sub>v xs frm to f acc obsv r' \<and>
+  "\<lbrakk>val_wa_foldnb_bod \<xi>\<^sub>v t xs frm (Suc to) f acc obsv r; Suc to \<le> length xs; frm < Suc to\<rbrakk>
+    \<Longrightarrow> \<exists>r'. val_wa_foldnb_bod \<xi>\<^sub>v t xs frm to f acc obsv r' \<and>
         (\<xi>\<^sub>v, [VRecord [xs ! to, r', obsv]] \<turnstile> (App f (Var 0)) \<Down> r)"
-  apply (induct arbitrary: 
-                rule: val_wa_foldnb_bod.induct[where ?a0.0 = \<xi>\<^sub>v and 
-                                                       ?a1.0 =xs and 
-                                                       ?a2.0 = frm and 
-                                                       ?a3.0 = to  and 
-                                                       ?a4.0 = f and
-                                                       ?a5.0 = acc and
-                                                       ?a6.0 = obsv and
-                                                       ?a7.0 = r]; clarsimp)
+  apply (induct rule: val_wa_foldnb_bod.induct[of _ \<xi>\<^sub>v t xs frm to f acc obsv r]; clarsimp)
   apply (erule val_wa_foldnb_bod.elims)
   apply (clarsimp split: if_split_asm)
   apply (erule_tac x = acc' in meta_allE)
@@ -1118,7 +1087,7 @@ lemma val_wa_foldnb_bod_back_step:
 
 
 lemma val_wa_foldnb_bod_preservation:
-  "\<lbrakk>proc_ctx_wellformed \<Xi>'; val.proc_env_matches \<xi>\<^sub>v \<Xi>'; val_wa_foldnb_bod \<xi>\<^sub>v xs frm to f acc obsv r; 
+  "\<lbrakk>proc_ctx_wellformed \<Xi>'; val.proc_env_matches \<xi>\<^sub>v \<Xi>'; val_wa_foldnb_bod \<xi>\<^sub>v t xs frm to f acc obsv r; 
     wa_abs_typing_v (VWA t xs) ''WordArray'' [t]; val.vval_typing \<Xi>' acc u; val.vval_typing \<Xi>' obsv v;
     \<Xi>', [], [option.Some (TRecord [(a0, (t, Present)), (a1, (u, Present)), 
       (a2, (v, Present))] Unboxed)] \<turnstile> App f (Var 0) : u; distinct [a0, a1, a2]\<rbrakk>
@@ -1145,6 +1114,210 @@ lemma val_wa_foldnb_bod_preservation:
   apply (rule val.v_t_r_empty)
   done
 
+function val_wa_mapAccumnb_bod :: "(char list, vatyp) vfoldmapdef"
+  where
+  "val_wa_mapAccumnb_bod \<xi>\<^sub>v t xs frm to f acc obsv res = 
+    (if frm < min to (length xs)
+      then (\<exists>v acc'. (\<xi>\<^sub>v, [(VRecord [xs ! frm, acc, obsv])] \<turnstile> App f (Var 0) \<Down> VRecord [v, acc']) \<and>
+          val_wa_mapAccumnb_bod \<xi>\<^sub>v t (xs[frm := v]) (Suc frm) to f acc' obsv res)
+    else res = VRecord [VAbstract (VWA t xs), acc])"
+  by pat_completeness auto
+termination
+  apply (relation "measure (\<lambda>(_, _, _, frm, to, _, _, _, _). to - frm)"; clarsimp)
+  apply linarith
+  done
+print_theorems
+declare val_wa_mapAccumnb_bod.simps[simp del]
+
+lemma val_wa_mapAccumnb_bod_to_geq_len:
+  "\<lbrakk>val_wa_mapAccumnb_bod \<xi>\<^sub>v t xs frm (length xs) f acc obsv r; length xs \<le> to\<rbrakk> 
+    \<Longrightarrow> val_wa_mapAccumnb_bod \<xi>\<^sub>v t xs frm to f acc obsv r"
+  apply (induct rule: val_wa_mapAccumnb_bod.induct[of _ \<xi>\<^sub>v t xs frm to f acc obsv r]; clarsimp)
+  apply (erule val_wa_mapAccumnb_bod.elims)
+  apply (clarsimp split: if_split_asm)
+   apply (erule_tac x = v in meta_allE)
+   apply (erule_tac x = acc' in meta_allE; clarsimp)
+   apply (subst val_wa_mapAccumnb_bod.simps)
+   apply clarsimp
+   apply (rule_tac x = v in exI)
+   apply (rule_tac x = acc' in exI)
+   apply clarsimp
+  apply (subst val_wa_mapAccumnb_bod.simps)
+  apply clarsimp
+  done
+
+lemma val_wa_mapAccumnb_bod_to_geq_lenD:
+  "\<lbrakk>val_wa_mapAccumnb_bod \<xi>\<^sub>v t xs frm to f acc obsv r; length xs \<le> to\<rbrakk> 
+    \<Longrightarrow> val_wa_mapAccumnb_bod \<xi>\<^sub>v t xs frm (length xs) f acc obsv r"
+  apply (induct rule: val_wa_mapAccumnb_bod.induct[of _ \<xi>\<^sub>v t xs frm to f acc obsv r]; clarsimp)
+  apply (erule val_wa_mapAccumnb_bod.elims)
+  apply (clarsimp split: if_split_asm)
+   apply (erule_tac x = v in meta_allE)
+   apply (erule_tac x = acc' in meta_allE; clarsimp)
+   apply (subst val_wa_mapAccumnb_bod.simps)
+   apply clarsimp
+   apply (rule_tac x = v in exI)
+   apply (rule_tac x = acc' in exI)
+   apply clarsimp
+  apply (subst val_wa_mapAccumnb_bod.simps)
+  apply clarsimp
+  done
+
+
+lemma val_wa_mapAccumnb_bod_step:
+  "\<lbrakk>val_wa_mapAccumnb_bod \<xi>\<^sub>v t xs frm to f acc obsv (VRecord [VAbstract (VWA t rxs), racc]); frm \<le> to;
+    to < length xs; \<xi>\<^sub>v, [VRecord [xs ! to, racc, obsv]] \<turnstile> (App f (Var 0)) \<Down> VRecord [v, racc']\<rbrakk> 
+    \<Longrightarrow> val_wa_mapAccumnb_bod \<xi>\<^sub>v t xs frm (Suc to) f acc obsv (VRecord [VAbstract (VWA t (rxs[to := v])), racc'])"
+  apply (induct arbitrary:rxs racc v racc'
+                rule: val_wa_mapAccumnb_bod.induct[of _ \<xi>\<^sub>v t xs frm to f acc obsv 
+                  "(VRecord [VAbstract (VWA t rxs), racc])"])
+  apply clarsimp
+  apply (erule val_wa_mapAccumnb_bod.elims)
+  apply (clarsimp split: if_split_asm)
+   apply (drule_tac x = va in meta_spec)
+   apply (drule_tac x = acc' in meta_spec)
+   apply (drule_tac x = rxs in meta_spec)
+   apply (drule_tac x = racc in meta_spec)
+   apply (drule_tac x = v in meta_spec)
+   apply (drule_tac x = racc' in meta_spec)
+   apply clarsimp
+   apply (subst val_wa_mapAccumnb_bod.simps)
+   apply clarsimp
+   apply (rule_tac x = va in exI)
+   apply (rule_tac x = acc' in exI)
+   apply clarsimp
+  apply (subst val_wa_mapAccumnb_bod.simps)
+  apply clarsimp
+  apply (rule_tac x = v in exI)
+  apply (rule_tac x = racc' in exI)
+  apply (subst val_wa_mapAccumnb_bod.simps)
+  apply clarsimp
+  done
+
+lemma val_wa_mapAccumnb_bod_back_step':
+  "\<lbrakk>val_wa_mapAccumnb_bod \<xi>\<^sub>v t xs frm (Suc to) f acc obsv r; length xs < Suc to\<rbrakk>
+    \<Longrightarrow> val_wa_mapAccumnb_bod \<xi>\<^sub>v t xs frm to f acc obsv r"
+  apply (induct rule: val_wa_mapAccumnb_bod.induct[of _ \<xi>\<^sub>v t xs frm to f acc obsv r]; clarsimp)
+  apply (erule val_wa_mapAccumnb_bod.elims)
+  apply (clarsimp split: if_split_asm)
+   apply (erule_tac x = v in meta_allE)
+   apply (erule_tac x = acc' in meta_allE; clarsimp)
+   apply (subst val_wa_mapAccumnb_bod.simps)
+   apply clarsimp
+   apply (rule_tac x = v in exI)
+   apply (rule_tac x = acc' in exI)
+   apply clarsimp
+  apply (subst val_wa_mapAccumnb_bod.simps)
+  apply clarsimp
+  done
+
+lemma val_wa_mapAccumnb_bod_back_step:
+  "\<lbrakk>val_wa_mapAccumnb_bod \<xi>\<^sub>v t xs frm (Suc to) f acc obsv (VRecord [VAbstract (VWA t rxs), racc]); 
+    Suc to \<le> length xs; frm < Suc to\<rbrakk>
+    \<Longrightarrow> \<exists>racc'.
+      val_wa_mapAccumnb_bod \<xi>\<^sub>v t xs frm to f acc obsv (VRecord [VAbstract (VWA t (rxs[to := xs ! to])), racc']) \<and>
+      (\<xi>\<^sub>v, [VRecord [xs ! to, racc', obsv]] \<turnstile> (App f (Var 0)) \<Down> VRecord [rxs ! to, racc])"
+  apply (induct arbitrary: rxs racc
+                rule: val_wa_mapAccumnb_bod.induct[of _ \<xi>\<^sub>v t xs frm to f acc obsv 
+                  "VRecord [VAbstract (VWA t rxs), racc]"])
+  apply clarsimp
+  apply (erule val_wa_mapAccumnb_bod.elims)
+  apply (clarsimp split: if_split_asm)
+  apply (erule_tac x = v in meta_allE)
+  apply (erule_tac x = acc' in meta_allE)
+  apply (erule_tac x = rxs in meta_allE)
+  apply (erule_tac x = racc in meta_allE)
+  apply clarsimp
+  apply (case_tac "frma < to")
+   apply clarsimp
+   apply (rule_tac x = racc' in exI)
+   apply clarsimp
+   apply (subst val_wa_mapAccumnb_bod.simps; clarsimp)
+   apply (rule_tac x = v in exI)
+   apply (rule_tac x = acc' in exI)
+   apply clarsimp
+  apply clarsimp
+  apply (subgoal_tac "to = frma")
+   apply clarsimp
+   apply (erule val_wa_mapAccumnb_bod.elims; clarsimp)
+   apply (rule_tac x = acca in exI; clarsimp)
+   apply (subst val_wa_mapAccumnb_bod.simps; clarsimp)
+  apply linarith
+  done
+
+lemma val_wa_mapAccumnb_bod_preservation':
+  "val_wa_mapAccumnb_bod \<xi>\<^sub>v t xs frm to f acc obsv r 
+    \<Longrightarrow> \<exists>rxs racc. r = VRecord [VAbstract(VWA t rxs), racc] \<and> length xs = length rxs"
+  apply (induct rule: val_wa_mapAccumnb_bod.induct[of _ \<xi>\<^sub>v t xs frm to f acc obsv r])
+  apply (erule val_wa_mapAccumnb_bod.elims; clarsimp split: if_split_asm)
+  done
+
+lemma val_wa_mapAccumnb_bod_preservation:
+  "\<lbrakk>proc_ctx_wellformed \<Xi>'; val.proc_env_matches \<xi>\<^sub>v \<Xi>'; val_wa_mapAccumnb_bod \<xi>\<^sub>v t xs frm to f acc obsv r; 
+    wa_abs_typing_v (VWA t xs) ''WordArray'' [t]; val.vval_typing \<Xi>' acc u; val.vval_typing \<Xi>' obsv v;
+    \<Xi>', [], [option.Some (TRecord [(a0, (t, Present)), (a1, (u, Present)), 
+      (a2, (v, Present))] Unboxed)] \<turnstile> App f (Var 0) : 
+      TRecord [(b0, (t, Present)), (b1, (u, Present))] Unboxed; 
+    distinct [a0, a1, a2]; distinct [b0, b1]\<rbrakk>
+    \<Longrightarrow> val.vval_typing \<Xi>' r (TRecord [
+      (b0, (TCon ''WordArray'' [t] (Boxed Writable ptrl), Present)),
+      (b1, (u, Present))] Unboxed)"
+  apply (induct to arbitrary: r)
+   apply (erule val_wa_mapAccumnb_bod.elims; clarsimp)
+   apply (rule val.v_t_record; simp?)
+   apply (rule val.v_t_r_cons1; simp?)
+    apply (rule val.v_t_abstract; simp)
+    apply (clarsimp simp: wa_abs_typing_v_def)
+    apply (case_tac t; clarsimp)
+   apply (rule val.v_t_r_cons1; simp?)
+   apply (rule val.v_t_r_empty)
+  apply (case_tac "length xs < Suc to")
+   apply (drule val_wa_mapAccumnb_bod_back_step'; simp)
+  apply (case_tac "Suc to \<le> frm")
+   apply (erule val_wa_mapAccumnb_bod.elims; clarsimp)
+   apply (rule val.v_t_record; simp?)
+   apply (rule val.v_t_r_cons1; simp?)
+    apply (rule val.v_t_abstract; simp)
+    apply (clarsimp simp: wa_abs_typing_v_def)
+    apply (case_tac t; clarsimp)
+   apply (rule val.v_t_r_cons1; simp?)
+   apply (rule val.v_t_r_empty)
+  apply (frule val_wa_mapAccumnb_bod_preservation'; clarsimp)
+  apply (drule val_wa_mapAccumnb_bod_back_step; clarsimp)
+  apply (drule_tac x = "VRecord [VAbstract (VWA t (rxs[to := xs ! to])), racc']" in meta_spec)
+  apply clarsimp
+  apply (erule val.v_t_recordE; clarsimp)
+  apply (erule val.v_t_r_consE; clarsimp)+
+  apply (erule val.v_t_r_emptyE; simp)
+   apply (drule_tac e = "App f (Var 0)" and
+      v = "VRecord [rxs ! to, racc]" and
+      \<gamma> = "[VRecord [xs ! to, racc', obsv]]" and
+      \<Gamma> = "[option.Some (TRecord [(a0, t, Present), (a1, u, Present), (a2, v, Present)] Unboxed)]" 
+      in val.preservation(1)[of "[]" "[]" _ _ _  \<xi>\<^sub>v, simplified]; simp?)
+  apply (clarsimp simp: val.matches_def)
+  apply (rule val.v_t_record; simp?)
+  apply (rule val.v_t_r_cons1)
+   apply (clarsimp simp: wa_abs_typing_v_def split: type.splits prim_type.splits)
+   apply (erule_tac x = to in allE; clarsimp)
+   apply (rule val.v_t_prim'; clarsimp)
+  apply (rule val.v_t_r_cons1; simp?)
+  apply (rule val.v_t_r_cons1; simp?)
+    apply (rule val.v_t_r_empty)
+   apply (erule val.v_t_recordE; clarsimp)
+   apply (erule val.v_t_r_consE; clarsimp)+
+   apply (erule val.v_t_r_emptyE; simp)
+  apply (rule val.v_t_abstractE; simp)
+  apply (rule val.v_t_record; simp)
+  apply (rule val.v_t_r_cons1)
+   apply (rule val.v_t_abstract; simp?)
+    apply (clarsimp simp: wa_abs_typing_v_def split: type.splits prim_type.splits)
+   apply (case_tac "i = to"; simp?)
+    apply (clarsimp simp: val.vval_typing.simps[of _ _ "TPrim _", simplified])
+   apply (erule_tac x = i in allE; clarsimp)+
+  apply (rule val.v_t_r_cons1; simp?)
+  apply (rule val.v_t_r_empty)
+  done
+
 fun is_vval_fun :: "('f, 'a) vval \<Rightarrow> bool"
   where
 "is_vval_fun (VFunction _ _) = True" |
@@ -1165,14 +1338,14 @@ definition val_wa_foldnb_0
       is_vval_fun func \<and> \<tau> = TRecord [(a0, t, Present), (a1, u, Present), (a2, v, Present)] Unboxed \<and>
       val.vval_typing \<Xi>' acc u \<and> val.vval_typing \<Xi>' obsv v \<and> 
       (\<Xi>', [], [option.Some \<tau>] \<turnstile> (App (vvalfun_to_exprfun func) (Var 0)) : u) \<and>
-      (val_wa_foldnb_bod \<xi>\<^sub>v xs (unat frm) (unat to) (vvalfun_to_exprfun func) acc obsv y))"
+      (val_wa_foldnb_bod \<xi>\<^sub>v t xs (unat frm) (unat to) (vvalfun_to_exprfun func) acc obsv y))"
 
 
 definition val_wa_foldnbp
   where
   "val_wa_foldnbp \<xi>\<^sub>p x y = (\<exists>t xs frm to func acc obsv. 
       x = VRecord [VAbstract (VWA t xs), VPrim (LU32 frm), VPrim (LU32 to), func, acc, obsv] \<and>
-      is_vval_fun func \<and> val_wa_foldnb_bod \<xi>\<^sub>p xs (unat frm) (unat to) (vvalfun_to_exprfun func) acc obsv y)"
+      is_vval_fun func \<and> val_wa_foldnb_bod \<xi>\<^sub>p t xs (unat frm) (unat to) (vvalfun_to_exprfun func) acc obsv y)"
 
 fun \<xi>m1 :: "(char list, vatyp) vabsfuns" 
   where
